formalisation/wfapScript.sml
@@ -1,0 +1,13 @@
+open HolKernel Parse boolLib bossLib;
+
+val _ = new_theory "wfap";
+
+
+Inductive wfap:
+wfap [] [] ∧
+wfap sl tl ⇒ wfab     
+
+
+
+val _ = export_theory();
+
